Prove helper functions by Codex

src/proof/kubernetes_model/common.v
@@ -1,5 +1,6 @@
 From New.proof Require Import prelude empty_ffi.
 From New.proof.kubernetes_model Require Export apimodel_init.
+From New.proof.k8s_io.apimachinery.pkg.apis.meta Require Import v1.
 From New.proof Require Export pure_objects.
 
 Section proof.
@@ -86,6 +87,1153 @@ Lemma wp_applyValidationAndDefaulting i l o (name : go_string) :
       ⌜ KObjectV.objectmeta o' = ((KObjectV.objectmeta o) <| ObjectMetaV.Generation' := W64 1 |>) ⌝ ∗
       ⌜ ObjectSpecV.created (KObjectV.spec o) (KObjectV.spec o') ⌝ ∗
       ⌜ ObjectStatusV.created (KObjectV.status o) (KObjectV.status o') ⌝
+  }}}.
+Proof.
+Admitted.
+
+Definition delete_preconditions_match (m : ObjectMetaV.t) (options : DeleteOptionsV.t) : Prop :=
+  match options.(DeleteOptionsV.Preconditions') with
+  | None => True
+  | Some preconditions =>
+      (match preconditions.(PreconditionsV.UID') with
+       | Some uid => uid = m.(ObjectMetaV.UID')
+       | None => True
+       end) ∧
+      (match preconditions.(PreconditionsV.ResourceVersion') with
+       | Some rv => rv = m.(ObjectMetaV.ResourceVersion')
+       | None => True
+       end)
+  end.
+
+Lemma wp_validateDeletePreconditions i l m options_l options dq (kind : go_string) :
+  {{{ is_pkg_init apimodel ∗
+      "%Hi" ∷ ⌜ i = interface.mk (ptrT.id v1.ObjectMeta.id) #l ⌝ ∗
+      "Hdeepown_m_l" ∷ ObjectMetaV.deepown_l l m dq ∗
+      "Hdeepown_options_l" ∷ DeleteOptionsV.deepown_l options_l options dq ∗
+      "%Hpre" ∷ ⌜ delete_preconditions_match m options ⌝
+  }}}
+    @! apimodel.validateDeletePreconditions #i #options_l #kind
+  {{{ RET #interface.nil;
+      ObjectMetaV.deepown_l l m dq ∗
+      DeleteOptionsV.deepown_l options_l options dq
+  }}}.
+Proof. (* This proof is fully written by Codex *)
+  wp_start as "H".
+  iNamed "H". subst i.
+  iDestruct "Hdeepown_options_l" as (coptions) "[Hoptions_l Hdeepown_options]".
+  iNamed "Hdeepown_options".
+  unfold delete_preconditions_match in Hpre.
+  destruct options.(DeleteOptionsV.Preconditions') as [preconditions|] eqn:Hpreconditions in Hpre |- *.
+  - iDestruct "Hdeepown_preconditions_some" as (cpreconditions) "[Hpreconditions_l Hdeepown_preconditions]".
+    iNamed "Hdeepown_preconditions".
+    assert (v1.DeleteOptions.Preconditions' coptions ≠ null) as Hpreconditions_not_null.
+    { intros Hnull.
+      apply (proj1 Hdeepown_preconditions_none) in Hnull.
+      congruence.
+    }
+    assert (bool_decide (v1.DeleteOptions.Preconditions' coptions = null) = false) as Hpreconditions_nonnull_decide.
+    { apply bool_decide_false. done. }
+    wp_auto.
+    rewrite Hpreconditions_nonnull_decide.
+    wp_auto.
+    destruct preconditions.(PreconditionsV.UID') as [uid|] eqn:Huid in Hpre |- *.
+    + destruct Hpre as [Huid_eq Hpre].
+      iDestruct "Hdeepown_uid_some" as (cuid) "[Huid_l ->]".
+      assert (v1.Preconditions.UID' cpreconditions ≠ null) as Huid_not_null.
+      { intros Hnull.
+        apply (proj1 Hdeepown_uid_none) in Hnull.
+        congruence.
+      }
+      assert (bool_decide (v1.Preconditions.UID' cpreconditions = null) = false) as Huid_nonnull_decide.
+      { apply bool_decide_false. done. }
+      rewrite Huid_nonnull_decide /=.
+      wp_auto.
+      wp_apply (v1.wp_GetUID_deepown with "[$Hdeepown_m_l]").
+      iIntros "Hdeepown_m_l".
+      rewrite Huid_eq. wp_auto.
+      rewrite bool_decide_true //. wp_auto.
+      destruct preconditions.(PreconditionsV.ResourceVersion') as [rv|] eqn:Hrv in Hpre |- *.
+      * rename Hpre into Hrv_eq.
+        iDestruct "Hdeepown_resourceversion_some" as (crv) "[Hrv_l ->]".
+        assert (v1.Preconditions.ResourceVersion' cpreconditions ≠ null) as Hrv_not_null.
+        { intros Hnull.
+          apply (proj1 Hdeepown_resourceversion_none) in Hnull.
+          congruence.
+        }
+        assert (bool_decide (v1.Preconditions.ResourceVersion' cpreconditions = null) = false) as Hrv_nonnull_decide.
+        { apply bool_decide_false. done. }
+        rewrite Hrv_nonnull_decide /=.
+        wp_auto.
+        wp_apply (v1.wp_GetResourceVersion_deepown with "[$Hdeepown_m_l]").
+        iIntros "Hdeepown_m_l".
+        rewrite Hrv_eq. wp_auto.
+        rewrite bool_decide_true //. wp_auto.
+        iAssert ((match preconditions.(PreconditionsV.UID') with
+          | Some vu => ∃ cu, v1.Preconditions.UID' cpreconditions ↦{dq} cu ∗ ⌜ cu = vu ⌝
+          | None => True
+          end)%I) with "[Huid_l]" as "Huid_some_packed".
+        { rewrite Huid /=. iExists (ObjectMetaV.UID' m). iFrame "Huid_l". iPureIntro. symmetry. done. }
+        iAssert ((match preconditions.(PreconditionsV.ResourceVersion') with
+          | Some vrv => ∃ crv, v1.Preconditions.ResourceVersion' cpreconditions ↦{dq} crv ∗ ⌜ crv = vrv ⌝
+          | None => True
+          end)%I) with "[Hrv_l]" as "Hrv_some_packed".
+        { rewrite Hrv /=. iExists (ObjectMetaV.ResourceVersion' m). iFrame "Hrv_l". iPureIntro. symmetry. done. }
+        iAssert (PreconditionsV.deepown cpreconditions preconditions dq)
+          with "[Huid_some_packed Hrv_some_packed]" as "Hpreconditions_packed".
+        { rewrite /PreconditionsV.deepown Huid Hrv /=. iFrame. iPureIntro. done. }
+        iAssert ((match options.(DeleteOptionsV.Preconditions') with
+          | Some vp =>
+              ∃ cp, v1.DeleteOptions.Preconditions' coptions ↦{dq} cp ∗ PreconditionsV.deepown cp vp dq
+          | None => True
+          end)%I) with "[Hpreconditions_l Hpreconditions_packed]" as "Hpreconditions_some_packed".
+        { rewrite Hpreconditions /=. iExists cpreconditions. iFrame "Hpreconditions_l Hpreconditions_packed". }
+        iApply "HΦ".
+        iFrame "Hdeepown_m_l".
+        iExists coptions.
+        iFrame.
+        iPureIntro.
+        done.
+      * assert (v1.Preconditions.ResourceVersion' cpreconditions = null) as Hrv_null.
+        { apply (proj2 Hdeepown_resourceversion_none). done. }
+        rewrite bool_decide_true //=.
+        wp_auto.
+        iAssert ((match preconditions.(PreconditionsV.UID') with
+          | Some vu => ∃ cu, v1.Preconditions.UID' cpreconditions ↦{dq} cu ∗ ⌜ cu = vu ⌝
+          | None => True
+          end)%I) with "[Huid_l]" as "Huid_some_packed".
+        { rewrite Huid /=. iExists (ObjectMetaV.UID' m). iFrame "Huid_l". iPureIntro. symmetry. done. }
+        iAssert ((match preconditions.(PreconditionsV.ResourceVersion') with
+          | Some vrv => ∃ crv, v1.Preconditions.ResourceVersion' cpreconditions ↦{dq} crv ∗ ⌜ crv = vrv ⌝
+          | None => True
+          end)%I) as "Hrv_some_packed".
+        { rewrite Hrv /=. done. }
+        iAssert (PreconditionsV.deepown cpreconditions preconditions dq)
+          with "[Huid_some_packed Hrv_some_packed]" as "Hpreconditions_packed".
+        { rewrite /PreconditionsV.deepown Huid Hrv /=. iFrame. iPureIntro. done. }
+        iAssert ((match options.(DeleteOptionsV.Preconditions') with
+          | Some vp =>
+              ∃ cp, v1.DeleteOptions.Preconditions' coptions ↦{dq} cp ∗ PreconditionsV.deepown cp vp dq
+          | None => True
+          end)%I) with "[Hpreconditions_l Hpreconditions_packed]" as "Hpreconditions_some_packed".
+        { rewrite Hpreconditions /=. iExists cpreconditions. iFrame "Hpreconditions_l Hpreconditions_packed". }
+        iApply "HΦ".
+        iFrame "Hdeepown_m_l".
+        iExists coptions.
+        iFrame.
+        iPureIntro.
+        done.
+    + destruct Hpre as [_ Hpre].
+      assert (v1.Preconditions.UID' cpreconditions = null) as Huid_null.
+      { apply (proj2 Hdeepown_uid_none). done. }
+      rewrite bool_decide_true //=.
+      wp_auto.
+      destruct preconditions.(PreconditionsV.ResourceVersion') as [rv|] eqn:Hrv in Hpre |- *.
+      * rename Hpre into Hrv_eq.
+        iDestruct "Hdeepown_resourceversion_some" as (crv) "[Hrv_l ->]".
+        assert (v1.Preconditions.ResourceVersion' cpreconditions ≠ null) as Hrv_not_null.
+        { intros Hnull.
+          apply (proj1 Hdeepown_resourceversion_none) in Hnull.
+          congruence.
+        }
+        assert (bool_decide (v1.Preconditions.ResourceVersion' cpreconditions = null) = false) as Hrv_nonnull_decide.
+        { apply bool_decide_false. done. }
+        rewrite Hrv_nonnull_decide /=.
+        wp_auto.
+        wp_apply (v1.wp_GetResourceVersion_deepown with "[$Hdeepown_m_l]").
+        iIntros "Hdeepown_m_l".
+        rewrite Hrv_eq. wp_auto.
+        rewrite bool_decide_true //. wp_auto.
+        iAssert ((match preconditions.(PreconditionsV.UID') with
+          | Some vu => ∃ cu, v1.Preconditions.UID' cpreconditions ↦{dq} cu ∗ ⌜ cu = vu ⌝
+          | None => True
+          end)%I) as "Huid_some_packed".
+        { rewrite Huid /=. done. }
+        iAssert ((match preconditions.(PreconditionsV.ResourceVersion') with
+          | Some vrv => ∃ crv, v1.Preconditions.ResourceVersion' cpreconditions ↦{dq} crv ∗ ⌜ crv = vrv ⌝
+          | None => True
+          end)%I) with "[Hrv_l]" as "Hrv_some_packed".
+        { rewrite Hrv /=. iExists (ObjectMetaV.ResourceVersion' m). iFrame "Hrv_l". iPureIntro. symmetry. done. }
+        iAssert (PreconditionsV.deepown cpreconditions preconditions dq)
+          with "[Huid_some_packed Hrv_some_packed]" as "Hpreconditions_packed".
+        { rewrite /PreconditionsV.deepown Huid Hrv /=. iFrame. iPureIntro. done. }
+        iAssert ((match options.(DeleteOptionsV.Preconditions') with
+          | Some vp =>
+              ∃ cp, v1.DeleteOptions.Preconditions' coptions ↦{dq} cp ∗ PreconditionsV.deepown cp vp dq
+          | None => True
+          end)%I) with "[Hpreconditions_l Hpreconditions_packed]" as "Hpreconditions_some_packed".
+        { rewrite Hpreconditions /=. iExists cpreconditions. iFrame "Hpreconditions_l Hpreconditions_packed". }
+        iApply "HΦ".
+        iFrame "Hdeepown_m_l".
+        iExists coptions.
+        iFrame.
+        iPureIntro.
+        done.
+      * assert (v1.Preconditions.ResourceVersion' cpreconditions = null) as Hrv_null.
+        { apply (proj2 Hdeepown_resourceversion_none). done. }
+        rewrite bool_decide_true //=.
+        wp_auto.
+        iAssert ((match preconditions.(PreconditionsV.UID') with
+          | Some vu => ∃ cu, v1.Preconditions.UID' cpreconditions ↦{dq} cu ∗ ⌜ cu = vu ⌝
+          | None => True
+          end)%I) as "Huid_some_packed".
+        { rewrite Huid /=. done. }
+        iAssert ((match preconditions.(PreconditionsV.ResourceVersion') with
+          | Some vrv => ∃ crv, v1.Preconditions.ResourceVersion' cpreconditions ↦{dq} crv ∗ ⌜ crv = vrv ⌝
+          | None => True
+          end)%I) as "Hrv_some_packed".
+        { rewrite Hrv /=. done. }
+        iAssert (PreconditionsV.deepown cpreconditions preconditions dq)
+          with "[Huid_some_packed Hrv_some_packed]" as "Hpreconditions_packed".
+        { rewrite /PreconditionsV.deepown Huid Hrv /=. iFrame. iPureIntro. done. }
+        iAssert ((match options.(DeleteOptionsV.Preconditions') with
+          | Some vp =>
+              ∃ cp, v1.DeleteOptions.Preconditions' coptions ↦{dq} cp ∗ PreconditionsV.deepown cp vp dq
+          | None => True
+          end)%I) with "[Hpreconditions_l Hpreconditions_packed]" as "Hpreconditions_some_packed".
+        { rewrite Hpreconditions /=. iExists cpreconditions. iFrame "Hpreconditions_l Hpreconditions_packed". }
+        iApply "HΦ".
+        iFrame "Hdeepown_m_l".
+        iExists coptions.
+        iFrame.
+        iPureIntro.
+        done.
+  - assert (v1.DeleteOptions.Preconditions' coptions = null) as Hpreconditions_null.
+    { apply (proj2 Hdeepown_preconditions_none). done. }
+    wp_auto.
+    rewrite bool_decide_true //.
+    wp_auto.
+    iApply "HΦ".
+    iFrame "Hdeepown_m_l".
+    iExists coptions.
+    rewrite /DeleteOptionsV.deepown Hpreconditions /=.
+    iFrame.
+    iPureIntro.
+    done.
+Qed.
+
+Axiom delete_propagation_orphan_eq :
+  v1.DeletePropagationOrphan = #("Orphan"%go).
+
+Axiom delete_propagation_foreground_eq :
+  v1.DeletePropagationForeground = #("Foreground"%go).
+
+Axiom delete_propagation_background_eq :
+  v1.DeletePropagationBackground = #("Background"%go).
+
+Axiom finalizer_orphan_dependents_eq :
+  v1.FinalizerOrphanDependents = "orphan"%go.
+
+Axiom finalizer_delete_dependents_eq :
+  v1.FinalizerDeleteDependents = "foregroundDeletion"%go.
+
+Lemma wp_checkGracefulDelete
+    (kind : go_string) (i : interface.t) (o : KObjectV.t)
+    (options_l : loc) (options : DeleteOptionsV.t) :
+  {{{ is_pkg_init apimodel ∗
+      "Hdeepown_i" ∷ KObjectV.deepown_i i o 1 ∗
+      "Hdeepown_options_l" ∷ DeleteOptionsV.deepown_l options_l options 1
+  }}}
+    @! apimodel.checkGracefulDelete #kind #i #options_l
+  {{{ (graceful pendingGraceful : bool) (err : error.t) (o' : KObjectV.t)
+      (options' : DeleteOptionsV.t), RET (#graceful, #pendingGraceful, #err);
+      KObjectV.deepown_i i o' 1 ∗
+      DeleteOptionsV.deepown_l options_l options' 1 ∗
+      ⌜ pendingGraceful = true →
+          (KObjectV.objectmeta o').(ObjectMetaV.DeletionTimestamp') ≠ None ⌝
+  }}}.
+Proof.
+Admitted.
+
+Lemma wp_shouldOrphanDependents
+    (metadata_i : interface.t) (metadata_l : loc) (m : ObjectMetaV.t)
+    (options_l : loc) (options : DeleteOptionsV.t) (dq : dfrac) :
+  {{{ is_pkg_init apimodel ∗
+      "%Hmetadata" ∷ ⌜ metadata_i = interface.mk (ptrT.id v1.ObjectMeta.id) #metadata_l ⌝ ∗
+      "Hdeepown_m_l" ∷ ObjectMetaV.deepown_l metadata_l m dq ∗
+      "Hdeepown_options_l" ∷ DeleteOptionsV.deepown_l options_l options dq
+  }}}
+    @! apimodel.shouldOrphanDependents #metadata_i #options_l
+  {{{ (should_orphan : bool), RET #should_orphan;
+      ObjectMetaV.deepown_l metadata_l m dq ∗
+      DeleteOptionsV.deepown_l options_l options dq
+  }}}.
+Proof. (* This proof is fully written by Codex *)
+  wp_start as "H".
+  iNamed "H". subst metadata_i.
+  iDestruct "Hdeepown_m_l" as (cmeta) "[Hmeta_l Hdeepown_m]".
+  iDestruct "Hdeepown_options_l" as (coptions) "[Hoptions_l Hdeepown_options]".
+  iNamed "Hdeepown_m".
+  iNamed "Hdeepown_options".
+  iDestruct (typed_pointsto_not_null (t:=v1.DeleteOptions) with "Hoptions_l") as %Hoptions_not_null;
+    first (vm_compute; reflexivity).
+  assert (bool_decide (options_l = null) = false) as Hoptions_nonnull_decide.
+  { apply bool_decide_false. done. }
+  wp_auto.
+  destruct options.(DeleteOptionsV.PropagationPolicy') as [propagation_policy|] eqn:Hpropagation_policy.
+  - iDestruct "Hdeepown_propagationpolicy_some" as (cpropagation_policy) "[Hpropagation_policy_l ->]".
+    assert (v1.DeleteOptions.PropagationPolicy' coptions ≠ null) as Hpropagation_policy_not_null.
+    { intros Hnull.
+      apply (proj1 Hdeepown_propagationpolicy_none) in Hnull.
+      congruence.
+    }
+    assert (bool_decide (v1.DeleteOptions.PropagationPolicy' coptions = null) = false)
+      as Hpropagation_policy_nonnull_decide.
+    { apply bool_decide_false. done. }
+    rewrite Hoptions_nonnull_decide /=.
+    wp_auto.
+    rewrite Hpropagation_policy_nonnull_decide /=.
+    wp_auto.
+    rewrite delete_propagation_orphan_eq
+      delete_propagation_foreground_eq
+      delete_propagation_background_eq.
+    wp_auto.
+    destruct (bool_decide (propagation_policy = "Orphan"%go)) eqn:Hpropagation_policy_orphan.
+    + rewrite Hpropagation_policy_orphan. wp_auto.
+      iAssert (DeleteOptionsV.deepown_l options_l options dq) with
+        "[Hoptions_l Hdeepown_graceperiodseconds_some Hdeepown_preconditions_some
+          Hdeepown_orphandependents_some Hpropagation_policy_l]" as "Hdeepown_options_l".
+      { iExists coptions.
+        rewrite /DeleteOptionsV.deepown Hpropagation_policy /=.
+        iFrame.
+        iPureIntro.
+        done. }
+      iAssert (ObjectMetaV.deepown_l metadata_l m dq) with
+        "[Hmeta_l Hdeepown_creationtimestamp Hdeepown_deletiontimestamp_some
+          Hdeepown_deletiongraceperiodseconds_some Hdeepown_labels_some Hdeepown_annotations_some
+          Hdeepown_ownerreferences_some Hdeepown_finalizers_some Hdeepown_managedfields_some]" as "Hdeepown_m_l".
+      { iExists cmeta.
+        rewrite /ObjectMetaV.deepown /=.
+        iFrame.
+        iPureIntro.
+        done. }
+      iApply "HΦ".
+      iFrame.
+    + rewrite Hpropagation_policy_orphan. wp_auto.
+      destruct (bool_decide (propagation_policy = "Foreground"%go)) eqn:Hpropagation_policy_foreground.
+      * rewrite Hpropagation_policy_foreground. wp_auto.
+        iAssert (DeleteOptionsV.deepown_l options_l options dq) with
+          "[Hoptions_l Hdeepown_graceperiodseconds_some Hdeepown_preconditions_some
+            Hdeepown_orphandependents_some Hpropagation_policy_l]" as "Hdeepown_options_l".
+        { iExists coptions.
+          rewrite /DeleteOptionsV.deepown Hpropagation_policy /=.
+          iFrame.
+          iPureIntro.
+          done. }
+        iAssert (ObjectMetaV.deepown_l metadata_l m dq) with
+          "[Hmeta_l Hdeepown_creationtimestamp Hdeepown_deletiontimestamp_some
+            Hdeepown_deletiongraceperiodseconds_some Hdeepown_labels_some Hdeepown_annotations_some
+            Hdeepown_ownerreferences_some Hdeepown_finalizers_some Hdeepown_managedfields_some]" as "Hdeepown_m_l".
+        { iExists cmeta.
+          rewrite /ObjectMetaV.deepown /=.
+          iFrame.
+          iPureIntro.
+          done. }
+        iApply "HΦ".
+        iFrame.
+      * rewrite Hpropagation_policy_foreground. wp_auto.
+        destruct (bool_decide (propagation_policy = "Background"%go)) eqn:Hpropagation_policy_background.
+        -- rewrite Hpropagation_policy_background. wp_auto.
+           iAssert (DeleteOptionsV.deepown_l options_l options dq) with
+             "[Hoptions_l Hdeepown_graceperiodseconds_some Hdeepown_preconditions_some
+               Hdeepown_orphandependents_some Hpropagation_policy_l]" as "Hdeepown_options_l".
+           { iExists coptions.
+             rewrite /DeleteOptionsV.deepown Hpropagation_policy /=.
+             iFrame.
+             iPureIntro.
+             done. }
+           iAssert (ObjectMetaV.deepown_l metadata_l m dq) with
+             "[Hmeta_l Hdeepown_creationtimestamp Hdeepown_deletiontimestamp_some
+               Hdeepown_deletiongraceperiodseconds_some Hdeepown_labels_some Hdeepown_annotations_some
+               Hdeepown_ownerreferences_some Hdeepown_finalizers_some Hdeepown_managedfields_some]" as "Hdeepown_m_l".
+           { iExists cmeta.
+             rewrite /ObjectMetaV.deepown /=.
+             iFrame.
+             iPureIntro.
+             done. }
+           iApply "HΦ".
+           iFrame.
+        -- rewrite Hpropagation_policy_background. wp_auto.
+           iAssert (DeleteOptionsV.deepown_l options_l options dq) with
+             "[Hoptions_l Hdeepown_graceperiodseconds_some Hdeepown_preconditions_some
+               Hdeepown_orphandependents_some Hpropagation_policy_l]" as "Hdeepown_options_l".
+           { iExists coptions.
+             rewrite /DeleteOptionsV.deepown Hpropagation_policy /=.
+             iFrame.
+             iPureIntro.
+             done. }
+           destruct m.(ObjectMetaV.Finalizers') as [finalizers|] eqn:Hfinalizers.
+           --- iDestruct "Hdeepown_finalizers_some" as (cfinalizers) "[Hfinalizers_l ->]".
+               wp_apply (v1.wp_GetFinalizers with "[$Hmeta_l]").
+               iIntros "Hmeta_l".
+               wp_auto.
+               Transparent slice.for_range.
+               iDestruct (own_slice_len with "Hfinalizers_l") as %(Hfinalizers_len & Hfinalizers_nonneg).
+               set I := (∃ (i : w64) (f : go_string),
+                 "Hi_ptr" ∷ i_ptr ↦ i ∗
+                 "Hf_ptr" ∷ f_ptr ↦ f ∗
+                 "%Hi" ∷ ⌜ 0 ≤ sint.Z i ≤ sint.Z (slice.len_f (v1.ObjectMeta.Finalizers' cmeta)) ⌝
+               )%I.
+               iAssert (I) with "[i f]" as "Hloop_inv".
+               { iExists (W64 0), (default_val go_string).
+                 iFrame.
+                 iPureIntro.
+                 change (sint.Z (slice.len_f slice.nil)) with 0%Z.
+                 word. }
+               wp_for "Hloop_inv".
+               wp_if_destruct.
+               {
+                   wp_pure; first word.
+                   assert ((sint.nat i < length finalizers)%nat) as Hi_lookup.
+                   { rewrite Hfinalizers_len. word. }
+                   pose proof (list_lookup_lt finalizers (sint.nat i) Hi_lookup) as [this_finalizer Hlookup].
+                   wp_apply (wp_load_slice_elem with "[$Hfinalizers_l]").
+                   { word. }
+                   { iPureIntro. exact Hlookup. }
+                   iIntros "Hfinalizers_l".
+                   wp_auto.
+                   rewrite finalizer_orphan_dependents_eq
+                     finalizer_delete_dependents_eq.
+                   destruct (bool_decide (this_finalizer = "orphan"%go)) eqn:Hthis_finalizer_orphan.
+                   { wp_auto.
+                        wp_for_post.
+                        iAssert ((match m.(ObjectMetaV.Finalizers') with
+                          | Some vfs => ∃ cfs, cmeta.(v1.ObjectMeta.Finalizers') ↦*{dq} cfs ∗ ⌜ cfs = vfs ⌝
+                          | None => True
+                          end)%I) with "[Hfinalizers_l]" as "Hdeepown_finalizers_some".
+                        { rewrite Hfinalizers /=.
+                          iExists finalizers.
+                          iFrame "Hfinalizers_l".
+                          iPureIntro.
+                          done. }
+                        iAssert (ObjectMetaV.deepown_l metadata_l m dq) with
+                          "[Hmeta_l Hdeepown_creationtimestamp Hdeepown_deletiontimestamp_some
+                            Hdeepown_deletiongraceperiodseconds_some Hdeepown_labels_some Hdeepown_annotations_some
+                            Hdeepown_ownerreferences_some Hdeepown_finalizers_some Hdeepown_managedfields_some]" as "Hdeepown_m_l".
+                        { iExists cmeta.
+                          rewrite /ObjectMetaV.deepown Hfinalizers /=.
+                          iFrame.
+                          iPureIntro.
+                          done. }
+                        iApply "HΦ".
+                        iFrame.
+                   }
+                   { wp_auto.
+                        destruct (bool_decide (this_finalizer = "foregroundDeletion"%go)) eqn:Hthis_finalizer_delete.
+                        { wp_auto.
+                           wp_for_post.
+                           iAssert ((match m.(ObjectMetaV.Finalizers') with
+                             | Some vfs => ∃ cfs, cmeta.(v1.ObjectMeta.Finalizers') ↦*{dq} cfs ∗ ⌜ cfs = vfs ⌝
+                             | None => True
+                             end)%I) with "[Hfinalizers_l]" as "Hdeepown_finalizers_some".
+                           { rewrite Hfinalizers /=.
+                             iExists finalizers.
+                             iFrame "Hfinalizers_l".
+                             iPureIntro.
+                             done. }
+                           iAssert (ObjectMetaV.deepown_l metadata_l m dq) with
+                             "[Hmeta_l Hdeepown_creationtimestamp Hdeepown_deletiontimestamp_some
+                               Hdeepown_deletiongraceperiodseconds_some Hdeepown_labels_some Hdeepown_annotations_some
+                               Hdeepown_ownerreferences_some Hdeepown_finalizers_some Hdeepown_managedfields_some]" as "Hdeepown_m_l".
+                           { iExists cmeta.
+                             rewrite /ObjectMetaV.deepown Hfinalizers /=.
+                             iFrame.
+                             iPureIntro.
+                             done. }
+                           iApply "HΦ".
+                           iFrame.
+                        }
+                        { wp_auto.
+                           iApply wp_for_post_do.
+                           wp_auto.
+                           iFrame "Hdeepown_creationtimestamp Hdeepown_deletiontimestamp_some
+                             Hdeepown_deletiongraceperiodseconds_some Hdeepown_labels_some
+                             Hdeepown_annotations_some Hdeepown_ownerreferences_some Hfinalizers_l
+                             Hdeepown_managedfields_some HΦ options metadata finalizers
+                             Hdeepown_options_l Hmeta_l".
+                           iExists (word.add i (W64 1)), this_finalizer.
+                           iFrame.
+                           iPureIntro.
+                           word.
+                        }
+                   }
+               }
+               {
+                   iAssert ((match m.(ObjectMetaV.Finalizers') with
+                       | Some vfs => ∃ cfs, cmeta.(v1.ObjectMeta.Finalizers') ↦*{dq} cfs ∗ ⌜ cfs = vfs ⌝
+                       | None => True
+                       end)%I) with "[Hfinalizers_l]" as "Hdeepown_finalizers_some".
+                   { rewrite Hfinalizers /=.
+                     iExists finalizers.
+                     iFrame "Hfinalizers_l".
+                     iPureIntro.
+                     done. }
+                   iAssert (ObjectMetaV.deepown_l metadata_l m dq) with
+                     "[Hmeta_l Hdeepown_creationtimestamp Hdeepown_deletiontimestamp_some
+                       Hdeepown_deletiongraceperiodseconds_some Hdeepown_labels_some Hdeepown_annotations_some
+                       Hdeepown_ownerreferences_some Hdeepown_finalizers_some Hdeepown_managedfields_some]" as "Hdeepown_m_l".
+                   { iExists cmeta.
+                     rewrite /ObjectMetaV.deepown Hfinalizers /=.
+                     iFrame.
+                     iPureIntro.
+                     done. }
+                   iApply "HΦ".
+                   iFrame.
+               }
+           --- wp_apply (v1.wp_GetFinalizers with "[$Hmeta_l]").
+               iIntros "Hmeta_l".
+               assert (v1.ObjectMeta.Finalizers' cmeta = slice.nil) as Hfinalizers_nil.
+               { apply (proj2 Hdeepown_finalizers_none). done. }
+               wp_auto.
+               Transparent slice.for_range.
+               rewrite Hfinalizers_nil.
+               set I := (∃ (i : w64) (f : go_string),
+                 "Hi_ptr" ∷ i_ptr ↦ i ∗
+                 "Hf_ptr" ∷ f_ptr ↦ f ∗
+                 "%Hi" ∷ ⌜ 0 ≤ sint.Z i ≤ sint.Z (slice.len_f slice.nil) ⌝
+               )%I.
+               iAssert (I) with "[i f]" as "Hloop_inv".
+               { iExists (W64 0), (default_val go_string).
+                 iFrame.
+                 iPureIntro.
+                 assert (sint.Z (W64 0) = 0)%Z as -> by word.
+                 change (sint.Z (slice.len_f slice.nil)) with 0%Z.
+                 lia. }
+               wp_for "Hloop_inv".
+               wp_if_destruct.
+               { exfalso. word. }
+               {
+                 iAssert (ObjectMetaV.deepown_l metadata_l m dq) with
+                   "[Hmeta_l Hdeepown_creationtimestamp Hdeepown_deletiontimestamp_some
+                     Hdeepown_deletiongraceperiodseconds_some Hdeepown_labels_some Hdeepown_annotations_some
+                     Hdeepown_ownerreferences_some Hdeepown_managedfields_some]" as "Hdeepown_m_l".
+                 { iExists cmeta.
+                   rewrite /ObjectMetaV.deepown Hfinalizers /=.
+                   iFrame.
+                   iPureIntro.
+                   done. }
+                 iApply "HΦ".
+                 iFrame.
+               }
+  - assert (v1.DeleteOptions.PropagationPolicy' coptions = null) as Hpropagation_policy_null.
+    { apply (proj2 Hdeepown_propagationpolicy_none). done. }
+    rewrite Hoptions_nonnull_decide /=.
+    wp_auto.
+    rewrite bool_decide_true //=.
+    wp_auto.
+    iAssert (DeleteOptionsV.deepown_l options_l options dq) with
+      "[Hoptions_l Hdeepown_graceperiodseconds_some Hdeepown_preconditions_some
+        Hdeepown_orphandependents_some]" as "Hdeepown_options_l".
+    { iExists coptions.
+      rewrite /DeleteOptionsV.deepown Hpropagation_policy /=.
+      iFrame.
+      iPureIntro.
+      done. }
+    destruct m.(ObjectMetaV.Finalizers') as [finalizers|] eqn:Hfinalizers.
+    + iDestruct "Hdeepown_finalizers_some" as (cfinalizers) "[Hfinalizers_l ->]".
+      wp_apply (v1.wp_GetFinalizers with "[$Hmeta_l]").
+      iIntros "Hmeta_l".
+      wp_auto.
+      Transparent slice.for_range.
+      iDestruct (own_slice_len with "Hfinalizers_l") as %(Hfinalizers_len & Hfinalizers_nonneg).
+      set I := (∃ (i : w64) (f : go_string),
+        "Hi_ptr" ∷ i_ptr ↦ i ∗
+        "Hf_ptr" ∷ f_ptr ↦ f ∗
+        "%Hi" ∷ ⌜ 0 ≤ sint.Z i ≤ sint.Z (slice.len_f (v1.ObjectMeta.Finalizers' cmeta)) ⌝
+      )%I.
+      iAssert (I) with "[i f]" as "Hloop_inv".
+      { iExists (W64 0), (default_val go_string).
+        iFrame.
+        iPureIntro.
+        change (sint.Z (slice.len_f slice.nil)) with 0%Z.
+        word. }
+      wp_for "Hloop_inv".
+      wp_if_destruct.
+      {
+        wp_pure; first word.
+        assert ((sint.nat i < length finalizers)%nat) as Hi_lookup.
+        { rewrite Hfinalizers_len. word. }
+        pose proof (list_lookup_lt finalizers (sint.nat i) Hi_lookup) as [this_finalizer Hlookup].
+        wp_apply (wp_load_slice_elem with "[$Hfinalizers_l]").
+        { word. }
+        { iPureIntro. exact Hlookup. }
+        iIntros "Hfinalizers_l".
+        wp_auto.
+        rewrite finalizer_orphan_dependents_eq
+          finalizer_delete_dependents_eq.
+        destruct (bool_decide (this_finalizer = "orphan"%go)) eqn:Hthis_finalizer_orphan.
+        { wp_auto.
+          wp_for_post.
+          iAssert ((match m.(ObjectMetaV.Finalizers') with
+            | Some vfs => ∃ cfs, cmeta.(v1.ObjectMeta.Finalizers') ↦*{dq} cfs ∗ ⌜ cfs = vfs ⌝
+            | None => True
+            end)%I) with "[Hfinalizers_l]" as "Hdeepown_finalizers_some".
+          { rewrite Hfinalizers /=.
+            iExists finalizers.
+            iFrame "Hfinalizers_l".
+            iPureIntro.
+            done. }
+          iAssert (ObjectMetaV.deepown_l metadata_l m dq) with
+            "[Hmeta_l Hdeepown_creationtimestamp Hdeepown_deletiontimestamp_some
+              Hdeepown_deletiongraceperiodseconds_some Hdeepown_labels_some Hdeepown_annotations_some
+              Hdeepown_ownerreferences_some Hdeepown_finalizers_some Hdeepown_managedfields_some]" as "Hdeepown_m_l".
+          { iExists cmeta.
+            rewrite /ObjectMetaV.deepown Hfinalizers /=.
+            iFrame.
+            iPureIntro.
+            done. }
+          iApply "HΦ".
+          iFrame.
+        }
+        { wp_auto.
+          destruct (bool_decide (this_finalizer = "foregroundDeletion"%go)) eqn:Hthis_finalizer_delete.
+          { wp_auto.
+             wp_for_post.
+             iAssert ((match m.(ObjectMetaV.Finalizers') with
+               | Some vfs => ∃ cfs, cmeta.(v1.ObjectMeta.Finalizers') ↦*{dq} cfs ∗ ⌜ cfs = vfs ⌝
+               | None => True
+               end)%I) with "[Hfinalizers_l]" as "Hdeepown_finalizers_some".
+             { rewrite Hfinalizers /=.
+               iExists finalizers.
+               iFrame "Hfinalizers_l".
+               iPureIntro.
+               done. }
+             iAssert (ObjectMetaV.deepown_l metadata_l m dq) with
+               "[Hmeta_l Hdeepown_creationtimestamp Hdeepown_deletiontimestamp_some
+                 Hdeepown_deletiongraceperiodseconds_some Hdeepown_labels_some Hdeepown_annotations_some
+                 Hdeepown_ownerreferences_some Hdeepown_finalizers_some Hdeepown_managedfields_some]" as "Hdeepown_m_l".
+             { iExists cmeta.
+               rewrite /ObjectMetaV.deepown Hfinalizers /=.
+               iFrame.
+               iPureIntro.
+               done. }
+             iApply "HΦ".
+             iFrame.
+          }
+          { wp_auto.
+             iApply wp_for_post_do.
+             wp_auto.
+             iFrame "Hdeepown_creationtimestamp Hdeepown_deletiontimestamp_some
+               Hdeepown_deletiongraceperiodseconds_some Hdeepown_labels_some
+               Hdeepown_annotations_some Hdeepown_ownerreferences_some Hfinalizers_l
+               Hdeepown_managedfields_some HΦ options metadata finalizers
+               Hdeepown_options_l Hmeta_l".
+             iExists (word.add i (W64 1)), this_finalizer.
+             iFrame.
+             iPureIntro.
+             word.
+          }
+        }
+      }
+      {
+        iAssert ((match m.(ObjectMetaV.Finalizers') with
+            | Some vfs => ∃ cfs, cmeta.(v1.ObjectMeta.Finalizers') ↦*{dq} cfs ∗ ⌜ cfs = vfs ⌝
+            | None => True
+            end)%I) with "[Hfinalizers_l]" as "Hdeepown_finalizers_some".
+        { rewrite Hfinalizers /=.
+          iExists finalizers.
+          iFrame "Hfinalizers_l".
+          iPureIntro.
+          done. }
+        iAssert (ObjectMetaV.deepown_l metadata_l m dq) with
+          "[Hmeta_l Hdeepown_creationtimestamp Hdeepown_deletiontimestamp_some
+            Hdeepown_deletiongraceperiodseconds_some Hdeepown_labels_some Hdeepown_annotations_some
+            Hdeepown_ownerreferences_some Hdeepown_finalizers_some Hdeepown_managedfields_some]" as "Hdeepown_m_l".
+        { iExists cmeta.
+          rewrite /ObjectMetaV.deepown Hfinalizers /=.
+          iFrame.
+          iPureIntro.
+          done. }
+        iApply "HΦ".
+        iFrame.
+      }
+    + wp_apply (v1.wp_GetFinalizers with "[$Hmeta_l]").
+      iIntros "Hmeta_l".
+      assert (v1.ObjectMeta.Finalizers' cmeta = slice.nil) as Hfinalizers_nil.
+      { apply (proj2 Hdeepown_finalizers_none). done. }
+      wp_auto.
+      Transparent slice.for_range.
+      rewrite Hfinalizers_nil.
+      set I := (∃ (i : w64) (f : go_string),
+        "Hi_ptr" ∷ i_ptr ↦ i ∗
+        "Hf_ptr" ∷ f_ptr ↦ f ∗
+        "%Hi" ∷ ⌜ 0 ≤ sint.Z i ≤ sint.Z (slice.len_f slice.nil) ⌝
+      )%I.
+      iAssert (I) with "[i f]" as "Hloop_inv".
+      { iExists (W64 0), (default_val go_string).
+        iFrame.
+        iPureIntro.
+        assert (sint.Z (W64 0) = 0)%Z as -> by word.
+        change (sint.Z (slice.len_f slice.nil)) with 0%Z.
+        lia. }
+      wp_for "Hloop_inv".
+      wp_if_destruct.
+      { exfalso. word. }
+      {
+        iAssert (ObjectMetaV.deepown_l metadata_l m dq) with
+          "[Hmeta_l Hdeepown_creationtimestamp Hdeepown_deletiontimestamp_some
+            Hdeepown_deletiongraceperiodseconds_some Hdeepown_labels_some Hdeepown_annotations_some
+            Hdeepown_ownerreferences_some Hdeepown_managedfields_some]" as "Hdeepown_m_l".
+        { iExists cmeta.
+          rewrite /ObjectMetaV.deepown Hfinalizers /=.
+          iFrame.
+          iPureIntro.
+          done. }
+        iApply "HΦ".
+        iFrame.
+      }
+Qed.
+
+Lemma wp_shouldDeleteDependents
+    (metadata_i : interface.t) (metadata_l : loc) (m : ObjectMetaV.t)
+    (options_l : loc) (options : DeleteOptionsV.t) (dq : dfrac) :
+  {{{ is_pkg_init apimodel ∗
+      "%Hmetadata" ∷ ⌜ metadata_i = interface.mk (ptrT.id v1.ObjectMeta.id) #metadata_l ⌝ ∗
+      "Hdeepown_m_l" ∷ ObjectMetaV.deepown_l metadata_l m dq ∗
+      "Hdeepown_options_l" ∷ DeleteOptionsV.deepown_l options_l options dq
+  }}}
+    @! apimodel.shouldDeleteDependents #metadata_i #options_l
+  {{{ (should_delete : bool), RET #should_delete;
+      ObjectMetaV.deepown_l metadata_l m dq ∗
+      DeleteOptionsV.deepown_l options_l options dq
+  }}}.
+Proof. (* This proof is fully written by Codex *)
+  wp_start as "H".
+  iNamed "H". subst metadata_i.
+  iDestruct "Hdeepown_m_l" as (cmeta) "[Hmeta_l Hdeepown_m]".
+  iDestruct "Hdeepown_options_l" as (coptions) "[Hoptions_l Hdeepown_options]".
+  iNamed "Hdeepown_m".
+  iNamed "Hdeepown_options".
+  iDestruct (typed_pointsto_not_null (t:=v1.DeleteOptions) with "Hoptions_l") as %Hoptions_not_null;
+    first (vm_compute; reflexivity).
+  assert (bool_decide (options_l = null) = false) as Hoptions_nonnull_decide.
+  { apply bool_decide_false. done. }
+  wp_auto.
+  destruct options.(DeleteOptionsV.PropagationPolicy') as [propagation_policy|] eqn:Hpropagation_policy.
+  - iDestruct "Hdeepown_propagationpolicy_some" as (cpropagation_policy) "[Hpropagation_policy_l ->]".
+    assert (v1.DeleteOptions.PropagationPolicy' coptions ≠ null) as Hpropagation_policy_not_null.
+    { intros Hnull.
+      apply (proj1 Hdeepown_propagationpolicy_none) in Hnull.
+      congruence.
+    }
+    assert (bool_decide (v1.DeleteOptions.PropagationPolicy' coptions = null) = false)
+      as Hpropagation_policy_nonnull_decide.
+    { apply bool_decide_false. done. }
+    rewrite Hoptions_nonnull_decide /=.
+    wp_auto.
+    rewrite Hpropagation_policy_nonnull_decide /=.
+    wp_auto.
+    rewrite delete_propagation_orphan_eq
+      delete_propagation_foreground_eq
+      delete_propagation_background_eq.
+    wp_auto.
+    destruct (bool_decide (propagation_policy = "Foreground"%go)) eqn:Hpropagation_policy_foreground.
+    + rewrite Hpropagation_policy_foreground. wp_auto.
+      iAssert (DeleteOptionsV.deepown_l options_l options dq) with
+        "[Hoptions_l Hdeepown_graceperiodseconds_some Hdeepown_preconditions_some
+          Hdeepown_orphandependents_some Hpropagation_policy_l]" as "Hdeepown_options_l".
+      { iExists coptions.
+        rewrite /DeleteOptionsV.deepown Hpropagation_policy /=.
+        iFrame.
+        iPureIntro.
+        done. }
+      iAssert (ObjectMetaV.deepown_l metadata_l m dq) with
+        "[Hmeta_l Hdeepown_creationtimestamp Hdeepown_deletiontimestamp_some
+          Hdeepown_deletiongraceperiodseconds_some Hdeepown_labels_some Hdeepown_annotations_some
+          Hdeepown_ownerreferences_some Hdeepown_finalizers_some Hdeepown_managedfields_some]" as "Hdeepown_m_l".
+      { iExists cmeta.
+        rewrite /ObjectMetaV.deepown /=.
+        iFrame.
+        iPureIntro.
+        done. }
+      iApply "HΦ".
+      iFrame.
+    + rewrite Hpropagation_policy_foreground. wp_auto.
+      destruct (bool_decide (propagation_policy = "Orphan"%go)) eqn:Hpropagation_policy_orphan.
+      * rewrite Hpropagation_policy_orphan. wp_auto.
+        iAssert (DeleteOptionsV.deepown_l options_l options dq) with
+          "[Hoptions_l Hdeepown_graceperiodseconds_some Hdeepown_preconditions_some
+            Hdeepown_orphandependents_some Hpropagation_policy_l]" as "Hdeepown_options_l".
+        { iExists coptions.
+          rewrite /DeleteOptionsV.deepown Hpropagation_policy /=.
+          iFrame.
+          iPureIntro.
+          done. }
+        iAssert (ObjectMetaV.deepown_l metadata_l m dq) with
+          "[Hmeta_l Hdeepown_creationtimestamp Hdeepown_deletiontimestamp_some
+            Hdeepown_deletiongraceperiodseconds_some Hdeepown_labels_some Hdeepown_annotations_some
+            Hdeepown_ownerreferences_some Hdeepown_finalizers_some Hdeepown_managedfields_some]" as "Hdeepown_m_l".
+        { iExists cmeta.
+          rewrite /ObjectMetaV.deepown /=.
+          iFrame.
+          iPureIntro.
+          done. }
+        iApply "HΦ".
+        iFrame.
+      * rewrite Hpropagation_policy_orphan. wp_auto.
+        destruct (bool_decide (propagation_policy = "Background"%go)) eqn:Hpropagation_policy_background.
+        -- rewrite Hpropagation_policy_background. wp_auto.
+           iAssert (DeleteOptionsV.deepown_l options_l options dq) with
+             "[Hoptions_l Hdeepown_graceperiodseconds_some Hdeepown_preconditions_some
+               Hdeepown_orphandependents_some Hpropagation_policy_l]" as "Hdeepown_options_l".
+           { iExists coptions.
+             rewrite /DeleteOptionsV.deepown Hpropagation_policy /=.
+             iFrame.
+             iPureIntro.
+             done. }
+           iAssert (ObjectMetaV.deepown_l metadata_l m dq) with
+             "[Hmeta_l Hdeepown_creationtimestamp Hdeepown_deletiontimestamp_some
+               Hdeepown_deletiongraceperiodseconds_some Hdeepown_labels_some Hdeepown_annotations_some
+               Hdeepown_ownerreferences_some Hdeepown_finalizers_some Hdeepown_managedfields_some]" as "Hdeepown_m_l".
+           { iExists cmeta.
+             rewrite /ObjectMetaV.deepown /=.
+             iFrame.
+             iPureIntro.
+             done. }
+           iApply "HΦ".
+           iFrame.
+        -- rewrite Hpropagation_policy_background. wp_auto.
+           iAssert (DeleteOptionsV.deepown_l options_l options dq) with
+             "[Hoptions_l Hdeepown_graceperiodseconds_some Hdeepown_preconditions_some
+               Hdeepown_orphandependents_some Hpropagation_policy_l]" as "Hdeepown_options_l".
+           { iExists coptions.
+             rewrite /DeleteOptionsV.deepown Hpropagation_policy /=.
+             iFrame.
+             iPureIntro.
+             done. }
+           destruct m.(ObjectMetaV.Finalizers') as [finalizers|] eqn:Hfinalizers.
+           --- iDestruct "Hdeepown_finalizers_some" as (cfinalizers) "[Hfinalizers_l ->]".
+               wp_apply (v1.wp_GetFinalizers with "[$Hmeta_l]").
+               iIntros "Hmeta_l".
+               wp_auto.
+               Transparent slice.for_range.
+               iDestruct (own_slice_len with "Hfinalizers_l") as %(Hfinalizers_len & Hfinalizers_nonneg).
+               set I := (∃ (i : w64) (f : go_string),
+                 "Hi_ptr" ∷ i_ptr ↦ i ∗
+                 "Hf_ptr" ∷ f_ptr ↦ f ∗
+                 "%Hi" ∷ ⌜ 0 ≤ sint.Z i ≤ sint.Z (slice.len_f (v1.ObjectMeta.Finalizers' cmeta)) ⌝
+               )%I.
+               iAssert (I) with "[i f]" as "Hloop_inv".
+               { iExists (W64 0), (default_val go_string).
+                 iFrame.
+                 iPureIntro.
+                 word. }
+               wp_for "Hloop_inv".
+               wp_if_destruct.
+               {
+                 wp_pure; first word.
+                 assert ((sint.nat i < length finalizers)%nat) as Hi_lookup.
+                 { rewrite Hfinalizers_len. word. }
+                 pose proof (list_lookup_lt finalizers (sint.nat i) Hi_lookup) as [this_finalizer Hlookup].
+                 wp_apply (wp_load_slice_elem with "[$Hfinalizers_l]").
+                 { word. }
+                 { iPureIntro. exact Hlookup. }
+                 iIntros "Hfinalizers_l".
+                 wp_auto.
+                 rewrite finalizer_orphan_dependents_eq
+                   finalizer_delete_dependents_eq.
+                 destruct (bool_decide (this_finalizer = "foregroundDeletion"%go)) eqn:Hthis_finalizer_delete.
+                 { wp_auto.
+                   wp_for_post.
+                   iAssert ((match m.(ObjectMetaV.Finalizers') with
+                     | Some vfs => ∃ cfs, cmeta.(v1.ObjectMeta.Finalizers') ↦*{dq} cfs ∗ ⌜ cfs = vfs ⌝
+                     | None => True
+                     end)%I) with "[Hfinalizers_l]" as "Hdeepown_finalizers_some".
+                   { rewrite Hfinalizers /=.
+                     iExists finalizers.
+                     iFrame "Hfinalizers_l".
+                     iPureIntro.
+                     done. }
+                   iAssert (ObjectMetaV.deepown_l metadata_l m dq) with
+                     "[Hmeta_l Hdeepown_creationtimestamp Hdeepown_deletiontimestamp_some
+                       Hdeepown_deletiongraceperiodseconds_some Hdeepown_labels_some Hdeepown_annotations_some
+                       Hdeepown_ownerreferences_some Hdeepown_finalizers_some Hdeepown_managedfields_some]" as "Hdeepown_m_l".
+                   { iExists cmeta.
+                     rewrite /ObjectMetaV.deepown Hfinalizers /=.
+                     iFrame.
+                     iPureIntro.
+                     done. }
+                   iApply "HΦ".
+                   iFrame.
+                 }
+                 { wp_auto.
+                   destruct (bool_decide (this_finalizer = "orphan"%go)) eqn:Hthis_finalizer_orphan.
+                   { wp_auto.
+                     wp_for_post.
+                     iAssert ((match m.(ObjectMetaV.Finalizers') with
+                       | Some vfs => ∃ cfs, cmeta.(v1.ObjectMeta.Finalizers') ↦*{dq} cfs ∗ ⌜ cfs = vfs ⌝
+                       | None => True
+                       end)%I) with "[Hfinalizers_l]" as "Hdeepown_finalizers_some".
+                     { rewrite Hfinalizers /=.
+                       iExists finalizers.
+                       iFrame "Hfinalizers_l".
+                       iPureIntro.
+                       done. }
+                     iAssert (ObjectMetaV.deepown_l metadata_l m dq) with
+                       "[Hmeta_l Hdeepown_creationtimestamp Hdeepown_deletiontimestamp_some
+                         Hdeepown_deletiongraceperiodseconds_some Hdeepown_labels_some Hdeepown_annotations_some
+                         Hdeepown_ownerreferences_some Hdeepown_finalizers_some Hdeepown_managedfields_some]" as "Hdeepown_m_l".
+                     { iExists cmeta.
+                       rewrite /ObjectMetaV.deepown Hfinalizers /=.
+                       iFrame.
+                       iPureIntro.
+                       done. }
+                     iApply "HΦ".
+                     iFrame.
+                   }
+                   { wp_auto.
+                     iApply wp_for_post_do.
+                     wp_auto.
+                     iFrame "Hdeepown_creationtimestamp Hdeepown_deletiontimestamp_some
+                       Hdeepown_deletiongraceperiodseconds_some Hdeepown_labels_some
+                       Hdeepown_annotations_some Hdeepown_ownerreferences_some Hfinalizers_l
+                       Hdeepown_managedfields_some HΦ options metadata finalizers
+                       Hdeepown_options_l Hmeta_l".
+                     iExists (word.add i (W64 1)), this_finalizer.
+                     iFrame.
+                     iPureIntro.
+                     word.
+                   }
+                 }
+               }
+               {
+                 iAssert ((match m.(ObjectMetaV.Finalizers') with
+                     | Some vfs => ∃ cfs, cmeta.(v1.ObjectMeta.Finalizers') ↦*{dq} cfs ∗ ⌜ cfs = vfs ⌝
+                     | None => True
+                     end)%I) with "[Hfinalizers_l]" as "Hdeepown_finalizers_some".
+                 { rewrite Hfinalizers /=.
+                   iExists finalizers.
+                   iFrame "Hfinalizers_l".
+                   iPureIntro.
+                   done. }
+                 iAssert (ObjectMetaV.deepown_l metadata_l m dq) with
+                   "[Hmeta_l Hdeepown_creationtimestamp Hdeepown_deletiontimestamp_some
+                     Hdeepown_deletiongraceperiodseconds_some Hdeepown_labels_some Hdeepown_annotations_some
+                     Hdeepown_ownerreferences_some Hdeepown_finalizers_some Hdeepown_managedfields_some]" as "Hdeepown_m_l".
+                 { iExists cmeta.
+                   rewrite /ObjectMetaV.deepown Hfinalizers /=.
+                   iFrame.
+                   iPureIntro.
+                   done. }
+                 iApply "HΦ".
+                 iFrame.
+               }
+           --- wp_apply (v1.wp_GetFinalizers with "[$Hmeta_l]").
+               iIntros "Hmeta_l".
+               assert (v1.ObjectMeta.Finalizers' cmeta = slice.nil) as Hfinalizers_nil.
+               { apply (proj2 Hdeepown_finalizers_none). done. }
+               wp_auto.
+               Transparent slice.for_range.
+               rewrite Hfinalizers_nil.
+               set I := (∃ (i : w64) (f : go_string),
+                 "Hi_ptr" ∷ i_ptr ↦ i ∗
+                 "Hf_ptr" ∷ f_ptr ↦ f ∗
+                 "%Hi" ∷ ⌜ 0 ≤ sint.Z i ≤ sint.Z (slice.len_f slice.nil) ⌝
+               )%I.
+               iAssert (I) with "[i f]" as "Hloop_inv".
+               { iExists (W64 0), (default_val go_string).
+                 iFrame.
+                 iPureIntro.
+                 assert (sint.Z (W64 0) = 0)%Z as -> by word.
+                 change (sint.Z (slice.len_f slice.nil)) with 0%Z.
+                 lia. }
+               wp_for "Hloop_inv".
+               wp_if_destruct.
+               { exfalso. word. }
+               {
+                 iAssert (ObjectMetaV.deepown_l metadata_l m dq) with
+                   "[Hmeta_l Hdeepown_creationtimestamp Hdeepown_deletiontimestamp_some
+                     Hdeepown_deletiongraceperiodseconds_some Hdeepown_labels_some Hdeepown_annotations_some
+                     Hdeepown_ownerreferences_some Hdeepown_managedfields_some]" as "Hdeepown_m_l".
+                 { iExists cmeta.
+                   rewrite /ObjectMetaV.deepown Hfinalizers /=.
+                   iFrame.
+                   iPureIntro.
+                   done. }
+                 iApply "HΦ".
+                 iFrame.
+               }
+  - assert (v1.DeleteOptions.PropagationPolicy' coptions = null) as Hpropagation_policy_null.
+    { apply (proj2 Hdeepown_propagationpolicy_none). done. }
+    rewrite Hoptions_nonnull_decide /=.
+    wp_auto.
+    rewrite bool_decide_true //=.
+    wp_auto.
+    iAssert (DeleteOptionsV.deepown_l options_l options dq) with
+      "[Hoptions_l Hdeepown_graceperiodseconds_some Hdeepown_preconditions_some
+        Hdeepown_orphandependents_some]" as "Hdeepown_options_l".
+    { iExists coptions.
+      rewrite /DeleteOptionsV.deepown Hpropagation_policy /=.
+      iFrame.
+      iPureIntro.
+      done. }
+    destruct m.(ObjectMetaV.Finalizers') as [finalizers|] eqn:Hfinalizers.
+    + iDestruct "Hdeepown_finalizers_some" as (cfinalizers) "[Hfinalizers_l ->]".
+      wp_apply (v1.wp_GetFinalizers with "[$Hmeta_l]").
+      iIntros "Hmeta_l".
+      wp_auto.
+      Transparent slice.for_range.
+      iDestruct (own_slice_len with "Hfinalizers_l") as %(Hfinalizers_len & Hfinalizers_nonneg).
+      set I := (∃ (i : w64) (f : go_string),
+        "Hi_ptr" ∷ i_ptr ↦ i ∗
+        "Hf_ptr" ∷ f_ptr ↦ f ∗
+        "%Hi" ∷ ⌜ 0 ≤ sint.Z i ≤ sint.Z (slice.len_f (v1.ObjectMeta.Finalizers' cmeta)) ⌝
+      )%I.
+      iAssert (I) with "[i f]" as "Hloop_inv".
+      { iExists (W64 0), (default_val go_string).
+        iFrame.
+        iPureIntro.
+        word. }
+      wp_for "Hloop_inv".
+      wp_if_destruct.
+      {
+        wp_pure; first word.
+        assert ((sint.nat i < length finalizers)%nat) as Hi_lookup.
+        { rewrite Hfinalizers_len. word. }
+        pose proof (list_lookup_lt finalizers (sint.nat i) Hi_lookup) as [this_finalizer Hlookup].
+        wp_apply (wp_load_slice_elem with "[$Hfinalizers_l]").
+        { word. }
+        { iPureIntro. exact Hlookup. }
+        iIntros "Hfinalizers_l".
+        wp_auto.
+        rewrite finalizer_orphan_dependents_eq
+          finalizer_delete_dependents_eq.
+        destruct (bool_decide (this_finalizer = "foregroundDeletion"%go)) eqn:Hthis_finalizer_delete.
+        { wp_auto.
+          wp_for_post.
+          iAssert ((match m.(ObjectMetaV.Finalizers') with
+            | Some vfs => ∃ cfs, cmeta.(v1.ObjectMeta.Finalizers') ↦*{dq} cfs ∗ ⌜ cfs = vfs ⌝
+            | None => True
+            end)%I) with "[Hfinalizers_l]" as "Hdeepown_finalizers_some".
+          { rewrite Hfinalizers /=.
+            iExists finalizers.
+            iFrame "Hfinalizers_l".
+            iPureIntro.
+            done. }
+          iAssert (ObjectMetaV.deepown_l metadata_l m dq) with
+            "[Hmeta_l Hdeepown_creationtimestamp Hdeepown_deletiontimestamp_some
+              Hdeepown_deletiongraceperiodseconds_some Hdeepown_labels_some Hdeepown_annotations_some
+              Hdeepown_ownerreferences_some Hdeepown_finalizers_some Hdeepown_managedfields_some]" as "Hdeepown_m_l".
+          { iExists cmeta.
+            rewrite /ObjectMetaV.deepown Hfinalizers /=.
+            iFrame.
+            iPureIntro.
+            done. }
+          iApply "HΦ".
+          iFrame.
+        }
+        { wp_auto.
+          destruct (bool_decide (this_finalizer = "orphan"%go)) eqn:Hthis_finalizer_orphan.
+          { wp_auto.
+            wp_for_post.
+            iAssert ((match m.(ObjectMetaV.Finalizers') with
+              | Some vfs => ∃ cfs, cmeta.(v1.ObjectMeta.Finalizers') ↦*{dq} cfs ∗ ⌜ cfs = vfs ⌝
+              | None => True
+              end)%I) with "[Hfinalizers_l]" as "Hdeepown_finalizers_some".
+            { rewrite Hfinalizers /=.
+              iExists finalizers.
+              iFrame "Hfinalizers_l".
+              iPureIntro.
+              done. }
+            iAssert (ObjectMetaV.deepown_l metadata_l m dq) with
+              "[Hmeta_l Hdeepown_creationtimestamp Hdeepown_deletiontimestamp_some
+                Hdeepown_deletiongraceperiodseconds_some Hdeepown_labels_some Hdeepown_annotations_some
+                Hdeepown_ownerreferences_some Hdeepown_finalizers_some Hdeepown_managedfields_some]" as "Hdeepown_m_l".
+            { iExists cmeta.
+              rewrite /ObjectMetaV.deepown Hfinalizers /=.
+              iFrame.
+              iPureIntro.
+              done. }
+            iApply "HΦ".
+            iFrame.
+          }
+          { wp_auto.
+            iApply wp_for_post_do.
+            wp_auto.
+            iFrame "Hdeepown_creationtimestamp Hdeepown_deletiontimestamp_some
+              Hdeepown_deletiongraceperiodseconds_some Hdeepown_labels_some
+              Hdeepown_annotations_some Hdeepown_ownerreferences_some Hfinalizers_l
+              Hdeepown_managedfields_some HΦ options metadata finalizers
+              Hdeepown_options_l Hmeta_l".
+            iExists (word.add i (W64 1)), this_finalizer.
+            iFrame.
+            iPureIntro.
+            word.
+          }
+        }
+      }
+      {
+        iAssert ((match m.(ObjectMetaV.Finalizers') with
+            | Some vfs => ∃ cfs, cmeta.(v1.ObjectMeta.Finalizers') ↦*{dq} cfs ∗ ⌜ cfs = vfs ⌝
+            | None => True
+            end)%I) with "[Hfinalizers_l]" as "Hdeepown_finalizers_some".
+        { rewrite Hfinalizers /=.
+          iExists finalizers.
+          iFrame "Hfinalizers_l".
+          iPureIntro.
+          done. }
+        iAssert (ObjectMetaV.deepown_l metadata_l m dq) with
+          "[Hmeta_l Hdeepown_creationtimestamp Hdeepown_deletiontimestamp_some
+            Hdeepown_deletiongraceperiodseconds_some Hdeepown_labels_some Hdeepown_annotations_some
+            Hdeepown_ownerreferences_some Hdeepown_finalizers_some Hdeepown_managedfields_some]" as "Hdeepown_m_l".
+        { iExists cmeta.
+          rewrite /ObjectMetaV.deepown Hfinalizers /=.
+          iFrame.
+          iPureIntro.
+          done. }
+        iApply "HΦ".
+        iFrame.
+      }
+    + wp_apply (v1.wp_GetFinalizers with "[$Hmeta_l]").
+      iIntros "Hmeta_l".
+      assert (v1.ObjectMeta.Finalizers' cmeta = slice.nil) as Hfinalizers_nil.
+      { apply (proj2 Hdeepown_finalizers_none). done. }
+      wp_auto.
+      Transparent slice.for_range.
+      rewrite Hfinalizers_nil.
+      set I := (∃ (i : w64) (f : go_string),
+        "Hi_ptr" ∷ i_ptr ↦ i ∗
+        "Hf_ptr" ∷ f_ptr ↦ f ∗
+        "%Hi" ∷ ⌜ 0 ≤ sint.Z i ≤ sint.Z (slice.len_f slice.nil) ⌝
+      )%I.
+      iAssert (I) with "[i f]" as "Hloop_inv".
+      { iExists (W64 0), (default_val go_string).
+        iFrame.
+        iPureIntro.
+        assert (sint.Z (W64 0) = 0)%Z as -> by word.
+        change (sint.Z (slice.len_f slice.nil)) with 0%Z.
+        lia. }
+      wp_for "Hloop_inv".
+      wp_if_destruct.
+      { exfalso. word. }
+      {
+        iAssert (ObjectMetaV.deepown_l metadata_l m dq) with
+          "[Hmeta_l Hdeepown_creationtimestamp Hdeepown_deletiontimestamp_some
+            Hdeepown_deletiongraceperiodseconds_some Hdeepown_labels_some Hdeepown_annotations_some
+            Hdeepown_ownerreferences_some Hdeepown_managedfields_some]" as "Hdeepown_m_l".
+        { iExists cmeta.
+          rewrite /ObjectMetaV.deepown Hfinalizers /=.
+          iFrame.
+          iPureIntro.
+          done. }
+        iApply "HΦ".
+        iFrame.
+      }
+Qed.
+
+Lemma wp_State__deletionFinalizersForGarbageCollection
+    (l : loc) (metadata_i : interface.t) (metadata_l : loc) (m : ObjectMetaV.t)
+    (options_l : loc) (options : DeleteOptionsV.t) (dq : dfrac) (owner_uid : types.UID.t) :
+  {{{ is_pkg_init apimodel ∗
+      "%Hmetadata" ∷ ⌜ metadata_i = interface.mk (ptrT.id v1.ObjectMeta.id) #metadata_l ⌝ ∗
+      "Hdeepown_m_l" ∷ ObjectMetaV.deepown_l metadata_l m dq ∗
+      "Hdeepown_options_l" ∷ DeleteOptionsV.deepown_l options_l options dq
+  }}}
+    l @ (ptrT.id apimodel.State.id) @ "deletionFinalizersForGarbageCollection"
+      #metadata_i #options_l #owner_uid
+  {{{ (should_update_finalizers : bool) (new_finalizers_sl : slice.t),
+      RET (#should_update_finalizers, #new_finalizers_sl);
+      ObjectMetaV.deepown_l metadata_l m dq ∗
+      DeleteOptionsV.deepown_l options_l options dq
   }}}.
 Proof.
 Admitted.
